Updated Typing to add new context conversion premisses

pcuic/theories/PCUICTyping.v
@@ -23,7 +23,6 @@ Implicit Types (cf : checker_flags) (Σ : global_env_ext).
 
  *)
 
-
 Hint Rewrite subst_instance_length 
   fix_context_length fix_subst_length cofix_subst_length : len.
 
@@ -44,7 +43,6 @@ Definition extends (Σ Σ' : global_env) :=
   
 (** ** Typing relation *)
 
-Module PCUICEnvTyping := EnvTyping PCUICTerm PCUICEnvironment.
 Include PCUICEnvTyping.
 
 (* AXIOM GUARD CONDITION *)
@@ -269,6 +267,8 @@ Inductive typing `{checker_flags} (Σ : global_env_ext) (Γ : context) : term ->
     mdecl.(ind_npars) = ci.(ci_npar) ->
     let predctx := case_predicate_context ci.(ci_ind) mdecl idecl p in
     wf_predicate mdecl idecl p ->
+    wf_local Σ (Γ ,,, p.(pcontext)) ->
+    conv_context Σ (Γ ,,, p.(pcontext)) (Γ ,,, predctx) ->
     Σ ;;; Γ ,,, predctx |- p.(preturn) : tSort ps ->
     is_allowed_elimination Σ ps idecl.(ind_kelim) ->
     Σ ;;; Γ |- c : mkApps (tInd ci.(ci_ind) p.(puinst)) (p.(pparams) ++ indices) ->
@@ -277,7 +277,9 @@ Inductive typing `{checker_flags} (Σ : global_env_ext) (Γ : context) : term ->
     wf_branches idecl brs ->
     All2i (fun i cdecl br =>
       let brctxty := case_branch_type ci.(ci_ind) mdecl idecl p br ptm i cdecl in
-      ((Σ ;;; Γ ,,, brctxty.1 |- br.(bbody) : brctxty.2) *
+      (wf_local Σ (Γ ,,, br.(bcontext)) ×
+       conv_context Σ (Γ ,,, br.(bcontext)) (Γ ,,, brctxty.1)) ×
+      ((Σ ;;; Γ ,,, brctxty.1 |- br.(bbody) : brctxty.2) ×
       (Σ ;;; Γ ,,, brctxty.1 |- brctxty.2 : tSort ps))) 
       0 idecl.(ind_ctors) brs ->
     Σ ;;; Γ |- tCase ci p c brs : mkApps ptm (indices ++ [c])
@@ -351,12 +353,10 @@ Definition unlift_opt_pred (P : global_env_ext -> context -> option term -> term
   fun Σ Γ t T => P Σ Γ (Some t) T.
 
 
-Module PCUICTypingDef <: Typing PCUICTerm PCUICEnvironment PCUICEnvTyping.
+Module PCUICTypingDef <: Typing PCUICTerm PCUICEnvironment PCUICEnvTyping PCUICConversionPar PCUICConversion.
 
   Definition typing := @typing.
   Definition wf_universe := @wf_universe.
-  Definition conv := @conv.
-  Definition cumul := @cumul.
   Definition inds := inds. 
   Definition destArity := destArity [].
 End PCUICTypingDef.
@@ -366,6 +366,8 @@ Module PCUICDeclarationTyping :=
     PCUICTerm
     PCUICEnvironment
     PCUICEnvTyping
+    PCUICConversionPar
+    PCUICConversion
     PCUICTypingDef
     PCUICLookup.
 Include PCUICDeclarationTyping.
@@ -377,13 +379,18 @@ Definition tybranches {cf} Σ Γ ci mdecl idecl p ps ptm n ctors brs :=
    All2i
   (fun (i : nat) (cdecl : constructor_body) (br : branch term) =>
    let brctxty := case_branch_type ci mdecl idecl p br ptm i cdecl in
+   (wf_local Σ (Γ ,,, br.(bcontext)) × 
+    conv_context Σ (Γ ,,, br.(bcontext)) (Γ ,,, brctxty.1)) ×
    (Σ;;; Γ,,, brctxty.1 |- bbody br : brctxty.2
     × Σ;;; Γ,,, brctxty.1 |- brctxty.2 : tSort ps)) n ctors brs.
 
-Definition branches_size {cf} {Σ Γ ci mdecl idecl p ps ptm brs} (typing_size : forall Σ Γ t T, Σ ;;; Γ |- t : T -> size)
+Definition branches_size {cf} {Σ Γ ci mdecl idecl p ps ptm brs}
+   (typing_size : forall Σ Γ t T, Σ ;;; Γ |- t : T -> size)
   {n ctors}
   (a : tybranches Σ Γ ci mdecl idecl p ps ptm n ctors brs) : size :=
-  (all2i_size _ (fun i x y p => Nat.max (typing_size _ _ _ _ p.1) (typing_size _ _ _ _ p.2)) a).
+  (all2i_size _ (fun i x y p => 
+    Nat.max (wf_local_size _ typing_size _ p.1.1)
+      (Nat.max (typing_size _ _ _ _ p.2.1) (typing_size _ _ _ _ p.2.2))) a).
 
 Definition typing_size `{checker_flags} {Σ Γ t T} (d : Σ ;;; Γ |- t : T) : size.
 Proof.
@@ -408,7 +415,8 @@ Proof.
   - exact (S (S (wf_local_size _ typing_size _ a))).
   - exact (S (S (wf_local_size _ typing_size _ a))).
   - exact (S (S (wf_local_size _ typing_size _ a))).
-  - exact (S (Nat.max d1 (Nat.max d2 (branches_size typing_size a)))).
+  - exact (S (Nat.max (wf_local_size _ typing_size _ a) 
+      (Nat.max d1 (Nat.max d2 (branches_size typing_size a0))))).
   - exact (S (Nat.max (Nat.max (wf_local_size _ typing_size _ a) 
     (all_size _ (fun x p => typing_size Σ _ _ _ p.π2) a0)) (all_size _ (fun x p => typing_size Σ _ _ _ p) a1))).
   - exact (S (Nat.max (Nat.max (wf_local_size _ typing_size _ a) 
@@ -631,8 +639,6 @@ Lemma typing_ind_env_app_size `{cf : checker_flags} :
 
    (forall Σ (wfΣ : wf Σ.1) (Γ : context) (wfΓ : wf_local Σ Γ) (t : term) na A B u s,
        PΓ Σ Γ ->
-      
-
        Σ ;;; Γ |- tProd na A B : tSort s -> P Σ Γ (tProd na A B) (tSort s) ->
        forall (Ht : Σ ;;; Γ |- t : tProd na A B), P Σ Γ t (tProd na A B) ->
 
@@ -671,6 +677,8 @@ Lemma typing_ind_env_app_size `{cf : checker_flags} :
         mdecl.(ind_npars) = ci.(ci_npar) ->
         let predctx := case_predicate_context ci.(ci_ind) mdecl idecl p in
         wf_predicate mdecl idecl p ->
+        PΓ Σ (Γ ,,, p.(pcontext)) ->
+        conv_context Σ (Γ ,,, p.(pcontext)) (Γ ,,, predctx) ->
         forall pret : Σ ;;; Γ ,,, predctx |- p.(preturn) : tSort ps,
         P Σ (Γ ,,, predctx) p.(preturn) (tSort ps) ->
         PΓ Σ (Γ ,,, predctx) ->
@@ -682,6 +690,8 @@ Lemma typing_ind_env_app_size `{cf : checker_flags} :
         wf_branches idecl brs ->
         All2i (fun i cdecl br =>
           let brctxty := case_branch_type ci.(ci_ind) mdecl idecl p br ptm i cdecl in
+          (PΓ Σ (Γ ,,, br.(bcontext)) *
+           conv_context Σ (Γ ,,, br.(bcontext)) (Γ ,,, brctxty.1)) ×
           ((Σ ;;; Γ ,,, brctxty.1 |- br.(bbody) : brctxty.2) *
             PΓ Σ (Γ ,,, brctxty.1) *
             (P Σ (Γ ,,, brctxty.1) br.(bbody) brctxty.2 *
@@ -848,27 +858,28 @@ Proof.
     assert (Hdecls: typing_size H > 1 -> Forall_decls_typing P Σ.1).
     { specialize (X14 _ _ _  (type_Prop _)).
       simpl in X14. intros Hle. apply X14. lia. }
+    assert (Hwf : forall Γ' (Hwf : wf_local Σ Γ'),
+      wf_local_size _ (@typing_size _) _ Hwf < typing_size H ->
+      PΓ Σ Γ').
+    { intros. eapply (XΓ _ _ _ Hwf); auto.
+      clear -Pdecl wfΣ X14 H0.
+      revert Hwf H0.
+      induction Hwf; simpl in *; try destruct t2 as [u Hu]; simpl in *; constructor.
+      - simpl in *. apply IHHwf. lia.
+      - red. apply (X14 _ _ _ Hu). lia.
+      - simpl in *. apply IHHwf. lia.
+      - red. apply (X14 _ _ _ t3). lia.
+      - red. simpl. apply (X14 _ _ _ Hu). lia. }
 
-    assert (forall Γ' t T (Hty : Σ ;;; Γ' |- t : T),
+    assert (Htywf : forall Γ' t T (Hty : Σ ;;; Γ' |- t : T),
       typing_size Hty <= typing_size H ->
       PΓ Σ Γ').
-    { intros. eapply (XΓ _ _ _ (typing_wf_local Hty)); auto.
-      clear -Pdecl wfΣ X14 H0.
-      pose proof (typing_wf_local_size Hty).
-      set (foo := typing_wf_local Hty) in *.
-      clearbody foo. assert (wf_local_size Σ (@typing_size cf) Γ' foo < typing_size H) by lia.
-      clear H1 H0 Hty.
-      revert foo H2.
-      induction foo; simpl in *; try destruct t3 as [u Hu]; simpl in *; constructor.
-      - simpl in *. apply IHfoo. lia.
-      - red. apply (X14 _ _ _ Hu). lia.
-      - simpl in *. apply IHfoo. lia.
-      - red. apply (X14 _ _ _ t4). lia.
-      - red. simpl. apply (X14 _ _ _ Hu). lia. }
+    { intros. eapply (Hwf _ (typing_wf_local Hty)); auto.
+      pose proof (typing_wf_local_size Hty). lia. }
       
     clear IH.
     assert (pΓ : PΓ Σ Γ).
-    { apply (X13 _ _ _ H). lia. }
+    { apply (Htywf _ _ _ H). lia. }
     split; auto.
     set (wfΓ := typing_wf_local H); clearbody wfΓ.
     
@@ -902,29 +913,33 @@ Proof.
     -- eapply X7; eauto. apply Hdecls; simpl; lia.
 
     -- simpl in pΓ.
-        eapply (X8 Σ wfΣ Γ (typing_wf_local H0) ci); eauto.
-        ++ eapply (X14 _ _ _ H); eauto. simpl; auto with arith.
-        ++ eapply (X14 _ _ _ H); eauto. simpl; auto with arith.
-        ++ simpl in *. eapply (X13 _ _ _ H); eauto. clear. subst predctx. lia.
+       eapply (X8 Σ wfΣ Γ (typing_wf_local H0) ci); eauto.
+        ++ eapply (X14 _ _ _ H); eauto. rewrite /predctx. simpl. lia.
+        ++ eapply (Hwf _ a); simpl; lia.
+        ++ eapply (X14 _ _ _ H); eauto. rewrite /predctx; simpl; lia.
+        ++ eapply (Htywf _ _ _ H). rewrite /predctx; simpl; lia.
         ++ eapply (X14 _ _ _ H0); simpl. lia.
-        ++ clear Hdecls. simpl in X13. revert a X13 X14.
-          clear. intros. simpl in X14. clear w0.
-          simpl in X14.
-          subst ptm predctx; induction a.
+        ++ clear Hdecls. simpl in Hwf, Htywf, X14.
+          clear -Hwf Htywf X14. 
+          subst ptm predctx; induction a0.
           ** constructor.
-          ** destruct r0 as [? ?]. constructor.
+          ** destruct r0 as [[wfbctx convctx] [t t0]]. constructor.
               --- intros brctxty. 
                   repeat split.
+                  +++ apply (Hwf _ wfbctx). simpl. lia. 
+                  +++ apply convctx.
                   +++ exact t.
-                  +++ eapply (X13 _ _ _ t); eauto. simpl. lia.
+                  +++ eapply (Htywf _ _ _ t); eauto. simpl. lia.
                   +++ unshelve eapply (X14 _ _ _ t _); eauto.
                       simpl. lia.
                   +++ simpl; auto with arith.
                   +++ eapply (X14 _ _ _ t0); eauto. simpl; auto with arith.
                       lia.
-              --- apply IHa; auto. intros. apply (X13 _ _ _ Hty). simpl. lia.
+              --- apply IHa0; auto. intros. apply (X14 _ _ _ Hty). simpl. lia.
                   intros.
-                  eapply (X14 _ _ _ Hty). simpl. lia.
+                  eapply (Hwf _ Hwf0). simpl. lia.
+                  intros.
+                  eapply (Htywf _ _ _ Hty). simpl; lia.
 
     -- eapply X9; eauto. apply Hdecls; simpl.
         pose proof (typing_size_pos H). lia.
@@ -937,7 +952,7 @@ Proof.
                         S
                           (all_size _ (fun (x : def term) p => typing_size p) a1) ->
                         PΓ Σ Γ0).
-          {intros. eapply (X13 _ _ _ Hty); eauto. lia. }
+          {intros. eapply (Htywf _ _ _ Hty); eauto. lia. }
           destruct mfix. now rewrite nth_error_nil in e.
           depelim a1.
           eapply (X _ _ _ t). simpl. lia.
@@ -950,7 +965,7 @@ Proof.
                     typing_size p.π2) a0) ->
                     Forall_decls_typing P Σ.1 * P Σ Γ t T).
           intros; eauto. eapply (X14 _ _ _ Hty); eauto. simpl. lia.
-          clear X13 X14 a pΓ Hdecls.
+          clear Hwf Htywf X14 a pΓ Hdecls.
           clear -a0 X.
           induction a0; constructor.
           destruct p as [s Hs]. exists s; split; auto.
@@ -966,7 +981,7 @@ Proof.
                           (all_size _ (fun (x : def term) p => typing_size p) a1) ->
                         Forall_decls_typing P Σ.1 * P Σ Γ0 t T).
           {intros. eapply (X14 _ _ _ Hty); eauto. lia. }
-          clear X14 X13.
+          clear X14 Hwf Htywf.
           clear e decl i a0 Hdecls i0.
           remember (fix_context mfix) as mfixcontext. clear Heqmfixcontext.
 
@@ -983,7 +998,7 @@ Proof.
                         S
                           (all_size _ (fun (x : def term) p => typing_size p) a1) ->
                         PΓ Σ Γ0).
-          {intros. eapply (X13 _ _ _ Hty); eauto. lia. }
+          {intros. eapply (Htywf _ _ _ Hty); eauto. lia. }
           destruct mfix. now rewrite nth_error_nil in e.
           depelim a1.
           eapply (X _ _ _ t). simpl. lia.        
@@ -996,7 +1011,7 @@ Proof.
                   typing_size p.π2) a0) ->
                   Forall_decls_typing P Σ.1 * P Σ Γ t T).
         intros; eauto. eapply (X14 _ _ _ Hty); eauto. simpl; lia.
-        clear X13 X14 a pΓ Hdecls.
+        clear Hwf Htywf X14 a pΓ Hdecls.
         clear -a0 X.
         induction a0; constructor.
         destruct p as [s Hs]. exists s; split; auto.
@@ -1013,7 +1028,7 @@ Proof.
                                   (fun (x : def term) p => typing_size p) a1) ->
                       Forall_decls_typing P Σ.1 * P Σ Γ0 t T).
         {intros. eapply (X14 _ _ _ Hty); eauto. lia. }
-        clear X14 X13.
+        clear X14 Hwf Htywf.
         clear e decl i a0 Hdecls i0.
         remember (fix_context mfix) as mfixcontext. clear Heqmfixcontext.
 
@@ -1093,33 +1108,37 @@ Lemma typing_ind_env `{cf : checker_flags} :
         PΓ Σ Γ ->
         consistent_instance_ext Σ mdecl.(ind_universes) u ->
         P Σ Γ (tConstruct ind i u) (type_of_constructor mdecl cdecl (ind, i) u)) ->
-        (forall (Σ : global_env_ext) (wfΣ : wf Σ) (Γ : context) (wfΓ : wf_local Σ Γ),     
-        forall (ci : case_info) p c brs indices ps mdecl idecl
-          (isdecl : declared_inductive Σ.1 ci.(ci_ind) mdecl idecl),
-          Forall_decls_typing P Σ.1 -> 
-          PΓ Σ Γ ->
-          mdecl.(ind_npars) = ci.(ci_npar) ->
-          let predctx := case_predicate_context ci.(ci_ind) mdecl idecl p in
-          wf_predicate mdecl idecl p ->
-          forall pret : Σ ;;; Γ ,,, predctx |- p.(preturn) : tSort ps,
-          P Σ (Γ ,,, predctx) p.(preturn) (tSort ps) ->
-          PΓ Σ (Γ ,,, predctx) ->
-          is_allowed_elimination Σ ps idecl.(ind_kelim) ->
-          Σ ;;; Γ |- c : mkApps (tInd ci.(ci_ind) p.(puinst)) (p.(pparams) ++ indices) ->
-          P Σ Γ c (mkApps (tInd ci.(ci_ind) p.(puinst)) (p.(pparams) ++ indices)) ->
-          isCoFinite mdecl.(ind_finite) = false ->
-          let ptm := it_mkLambda_or_LetIn predctx p.(preturn) in
-          wf_branches idecl brs ->          
-          All2i (fun i cdecl br =>
-          let brctxty := case_branch_type ci.(ci_ind) mdecl idecl p br ptm i cdecl in
-          ((Σ ;;; Γ ,,, brctxty.1 |- br.(bbody) : brctxty.2) *
+        
+    (forall (Σ : global_env_ext) (wfΣ : wf Σ) (Γ : context) (wfΓ : wf_local Σ Γ),     
+      forall (ci : case_info) p c brs indices ps mdecl idecl
+      (isdecl : declared_inductive Σ.1 ci.(ci_ind) mdecl idecl),
+      Forall_decls_typing P Σ.1 -> 
+      PΓ Σ Γ ->
+      mdecl.(ind_npars) = ci.(ci_npar) ->
+      let predctx := case_predicate_context ci.(ci_ind) mdecl idecl p in
+      wf_predicate mdecl idecl p ->
+      PΓ Σ (Γ ,,, p.(pcontext)) ->
+      conv_context Σ (Γ ,,, p.(pcontext)) (Γ ,,, predctx) ->
+      forall pret : Σ ;;; Γ ,,, predctx |- p.(preturn) : tSort ps,
+      P Σ (Γ ,,, predctx) p.(preturn) (tSort ps) ->
+      PΓ Σ (Γ ,,, predctx) ->
+      is_allowed_elimination Σ ps idecl.(ind_kelim) ->
+      Σ ;;; Γ |- c : mkApps (tInd ci.(ci_ind) p.(puinst)) (p.(pparams) ++ indices) ->
+      P Σ Γ c (mkApps (tInd ci.(ci_ind) p.(puinst)) (p.(pparams) ++ indices)) ->
+      isCoFinite mdecl.(ind_finite) = false ->
+      let ptm := it_mkLambda_or_LetIn predctx p.(preturn) in
+      wf_branches idecl brs ->
+      All2i (fun i cdecl br =>
+        let brctxty := case_branch_type ci.(ci_ind) mdecl idecl p br ptm i cdecl in
+        (PΓ Σ (Γ ,,, br.(bcontext)) *
+          conv_context Σ (Γ ,,, br.(bcontext)) (Γ ,,, brctxty.1)) ×
+        ((Σ ;;; Γ ,,, brctxty.1 |- br.(bbody) : brctxty.2) *
           PΓ Σ (Γ ,,, brctxty.1) *
           (P Σ (Γ ,,, brctxty.1) br.(bbody) brctxty.2 *
-            ((Σ ;;; Γ ,,, brctxty.1 |- brctxty.2 : tSort ps) *
-              P Σ (Γ ,,, brctxty.1) brctxty.2 (tSort ps))))) 0 idecl.(ind_ctors) brs ->
-          P Σ Γ (tCase ci p c brs) (mkApps ptm (indices ++ [c]))) ->
-          
-
+          ((Σ ;;; Γ ,,, brctxty.1 |- brctxty.2 : tSort ps) *
+          P Σ (Γ ,,, brctxty.1) brctxty.2 (tSort ps))))) 0 idecl.(ind_ctors) brs ->
+      P Σ Γ (tCase ci p c brs) (mkApps ptm (indices ++ [c]))) ->
+      
     (forall Σ (wfΣ : wf Σ.1) (Γ : context) (wfΓ : wf_local Σ Γ) (p : projection) (c : term) u
           mdecl idecl pdecl (isdecl : declared_projection Σ.1 p mdecl idecl pdecl) args,
         Forall_decls_typing P Σ.1 -> PΓ Σ Γ ->
